\section{Additional Proofs and Derivations}

\paragraph{Derivation of the Full Procrustes Distance for Functional Data}
\label{app:deriv-full-proc-dist}
Consider two curves $\beta_1, \beta_2 : [0,1] \rightarrow \mathbb{C}$ with $\langle \beta_1, \mathbb{1} \rangle = \langle \beta_2, \mathbb{1} \rangle = 0$ where $\mathbb{1}$ is the constant function $\mathbb{1}(t) = 1$ for all $t \in [0,1]$.
Then $\beta_1$ and $\beta_2$ can be considered to be centered as
$$ \langle \beta_1, \mathbb{1} \rangle
= \int_0^1 \bar{\beta_1}(t)\mathbb{1}(t)dt\\
= \int_0^1 \bar{\beta_1}(t)dt
= \int_0^1 (y(t) + i x(t))dt
= \underbrace{\int_0^1 y(t)dt}_{\stackrel{!}{=}0} + i \underbrace{\int_0^1 x(t)dt}_{\stackrel{!}{=}0} = 0 $$

Then the full procrustes distance of $\beta_1, \beta_2$ is given by their minimum distance controlling for translation $\gamma \in \mathbb{C}$, and scaling and rotation $\omega = b e^{i\theta} \in \mathbb{C}$:
\begin{align*}
    d_F^2 =& \min_{\omega,\gamma \in \mathbb{C}} ||\beta_1 - \gamma \mathbb{1} - \omega \beta_2 ||^2 \\
    =& \min_{\omega,\gamma \in \mathbb{C}} \langle\beta_1 - \gamma \mathbb{1} - \omega \beta_2, \beta_1 - \gamma \mathbb{1} - \omega \beta_2 \rangle \\
    =& \min_{\omega,\gamma \in \mathbb{C}}
    \langle \beta_1 - \omega \beta_2, \beta_1 - \omega \beta_2 \rangle
    - \underbrace{\langle \beta_1, \gamma \mathbb{1} \rangle}_{=\,0}
    - \underbrace{\langle \gamma \mathbb{1}, \beta_1 \rangle}_{=\,0}
    + \underbrace{\langle \gamma \mathbb{1}, \omega \beta_2 \rangle}_{=\,0}
    + \underbrace{\langle \omega \beta_2, \gamma \mathbb{1} \rangle}_{=\,0}
    + \underbrace{\langle \gamma \mathbb{1}, \gamma \mathbb{1} \rangle}_{=||\gamma \mathbb{1}||^2} \\
    \stackrel{\gamma=0}{=}& \min_{\omega \in \mathbb{C}}\,
    \langle \beta_1, \beta_1 \rangle
    + \langle \omega \beta_2, \omega \beta_2 \rangle
    - \langle \beta_1, \omega \beta_2 \rangle
    - \langle \omega \beta_2, \beta_1 \rangle \\
    =& \min_{\omega \in \mathbb{C}}\,
    \langle \beta_1, \beta_1 \rangle
    + |\omega|^2 \langle \beta_2, \beta_2 \rangle
    - \omega \langle \beta_1, \beta_2 \rangle
    - \overline{\omega} \langle \beta_2, \beta_1 \rangle
\end{align*}
To find $\omega \in \mathbb{C}$ that minimizes $||\beta_1 - \omega \beta_2||^2$ we first consider the part of the problem dependent on $\theta$. We need to solve
$$ \min_{\omega \in \mathbb{C}}
- \omega \langle \beta_1, \beta_2 \rangle
- \overline{\omega} \langle \beta_2, \beta_1 \rangle  =
\max_{\omega \in \mathbb{C}}
\omega \langle \beta_1, \beta_2 \rangle
+ \overline{\omega} \langle \beta_2, \beta_1 \rangle $$
by using $\omega = b e^{i\theta}$ and $\langle \beta_1, \beta_2 \rangle = a e^{i\phi}$:
\begin{align*}
    \max_{\omega \in \mathbb{C}}
    \omega \langle \beta_1, \beta_2 \rangle
    + \overline{\omega} \langle \beta_2, \beta_1 \rangle
    =& \max_{b \in \mathbb{R}^+, \theta \in [0,2\pi]}
    b e^{i\theta} a e^{i\phi} + b e^{-i\theta} a e^{-i\phi} \\
    =& \max_{b \in \mathbb{R}^+, \theta \in [0,2\pi]}
    b e^{i\theta} a e^{i\phi} + b e^{-i\theta} a e^{-i\phi} \\
    =& \max_{b \in \mathbb{R}^+, \theta \in [0,2\pi]}
    2 b a \cos\left(\theta +\phi\right)\\
    \stackrel{\theta = -\phi}{=}& \max_{b \in \mathbb{R}^+}
    2 b a
\end{align*}
and using $\theta = -\phi$ the original mimization problem therefore simplifies to
\begin{align*}
    d_F^2 =&
    \min_{b \in \mathbb{R}^+}\,
    \langle \beta_1, \beta_1 \rangle
    + b^2 \langle \beta_2, \beta_2 \rangle
    - 2 b a \\
    \frac{\partial d_F^2}{\partial b} =& \,
    2 b \langle \beta_2, \beta_2 \rangle - 2a \stackrel{!}{=} 0 \\
    \Rightarrow \quad & b = \frac{a}{\langle \beta_2, \beta_2 \rangle}
\end{align*}
And for the \textit{full Procrustes distance} it follows that
$$ d_F^2
= \langle \beta_1, \beta_1 \rangle - \frac{a^2}{\langle \beta_2, \beta_2 \rangle}
= \langle \beta_1, \beta_1 \rangle - \frac{ \langle \beta_1, \beta_2 \rangle \langle \beta_2, \beta_1 \rangle}{\langle \beta_2, \beta_2 \rangle}$$
As this expression is not symmetric in $\beta_1$ and $\beta_2$ we can take the curves to be of unit length with $\tilde{\beta}_j = \frac{\beta_j}{||\beta_j||}$, $j=1,2$ with $||\beta_j|| = \sqrt{\langle \beta_j, \beta_j \rangle}$, so that $\langle \tilde\beta_1, \tilde\beta_1 \rangle = \langle \tilde\beta_2, \tilde\beta_2 \rangle = 1$ and obtain a suitable measure of distance:
$$ d_F = \sqrt{1 - \langle \tilde\beta_1, \tilde\beta_2 \rangle
\langle \tilde\beta_2, \tilde\beta_1 \rangle}
= \sqrt{1 - \frac{ \langle \beta_1, \beta_2 \rangle \langle \beta_2, \beta_1 \rangle}{\langle \beta_1, \beta_1 \rangle \langle \beta_2, \beta_2 \rangle}}$$


\section{Discussion of Possible Extensions to Closed Curves}

\section{Shape-Smoothing Using the Estimated Covariance-Surface}
